Coq metatheory builds

stlc_metatheory.v
@@ -1,141 +1,27 @@
-(* generated from: ../tests/test10st.ott *)
-
-Require Import List.  Require Import Arith.  Require Import Bool.
-(** syntax *)
-Definition termvar := nat.
-Lemma eq_termvar: forall (x y : termvar), {x = y} + {x <> y}.
-Proof.
-  decide equality.
-Defined.
-
-Definition typvar := nat.
-Lemma eq_typvar: forall (x y : typvar), {x = y} + {x <> y}.
-Proof.
-  decide equality.
-Defined.
-
-
-Inductive 
-T : Set := 
-   T_var : typvar -> T
- | T_arrow : T -> T -> T
-.
-
-Inductive 
-t : Set := 
-   t_Var : termvar -> t
- | t_Lam : termvar -> t -> t
- | t_App : t -> t -> t
-.
-
-Definition
-G : Set := list (termvar*T)
-.
-
-
-(** library functions *)
-Fixpoint list_mem (A:Set) (eq:forall a b:A,{a=b}+{a<>b}) (x:A) (l:list A) {struct l} : bool :=
-  match l with
-  | nil => false
-  | cons h t => if eq h x then true else list_mem A eq x t
-end.
-Implicit Arguments list_mem.
-
-Fixpoint list_minus (A:Set) (eq:forall a b:A,{a=b}+{a<>b}) (l1:list A) (l2:list A) {struct l1} : list A :=
-  match l1 with
-  | nil => nil
-  | cons h t => if (list_mem (A:=A) eq h l2) then list_minus A eq t l2 else cons h (list_minus A eq t l2)
-end.
-Implicit Arguments list_minus.
-
-
-(** subrules *)
-Definition is_v_of_t (t_6:t) : Prop :=
-  match t_6 with
-  | (t_Var x) => False
-  | (t_Lam x t5) => (True)
-  | (t_App t5 t') => False
-end.
-
-
-(** free variables *)
-Fixpoint fv_t (t_6:t) : list termvar :=
-  match t_6 with
-  | (t_Var x) => ((cons x nil))
-  | (t_Lam x t5) => ((list_minus eq_termvar (fv_t t5) (cons x nil)))
-  | (t_App t5 t') => (app (fv_t t5) (fv_t t'))
-end.
-
-
-(** substitutions *)
-Fixpoint tsubst_t (t_6:t) (x5:termvar) (t__7:t) {struct t__7} : t :=
-  match t__7 with
-  | (t_Var x) => (if eq_termvar x x5 then t_6 else (t_Var x))
-  | (t_Lam x t5) => t_Lam x (if list_mem eq_termvar x5 (cons x nil) then t5 else (tsubst_t t_6 x5 t5))
-  | (t_App t5 t') => t_App (tsubst_t t_6 x5 t5) (tsubst_t t_6 x5 t')
-end.
-
-
-(** definitions *)
-(* defns Jtype *)
-
-Inductive
-(* defn GtT *)
-
-GtT : G -> t -> T -> Prop :=
- | GtT_value_name : forall G5 x T5,
-      (exists G1, exists G2, (( G5  = (app G1 (cons ( x , T5 )  G2 ))) /\ not (In  x  (List.map (fun (h:termvar*T) => match h with (h1,h2) => h1 end) G1))))  ->
-     GtT G5 (t_Var x) T5
- | GtT_apply : forall G5 t5 t' T2 T1,
-     GtT G5 t5 (T_arrow T1 T2) ->
-     GtT G5 t' T1 ->
-     GtT G5 (t_App t5 t') T2
- | GtT_lambda : forall G5 x1 t5 T1 T_5,
-     GtT  (cons ( x1 , T1 )  G5 )  t5 T_5 ->
-     GtT G5 (t_Lam x1 t5) (T_arrow T1 T_5)
-
-.
-(* defns Jop *)
-
-Inductive
-(* defn reduce *)
-
-reduce : t -> t -> Prop :=
- | ax_app : forall x t12 v2,
-     is_v_of_t v2 ->
-     reduce (t_App  (t_Lam x t12)  v2)  ( tsubst_t  v2   x   t12  ) 
- | ctx_app_fun : forall t1 t_5 t1',
-     reduce t1 t1' ->
-     reduce (t_App t1 t_5) (t_App t1' t_5)
- | ctx_app_arg : forall v5 t1 t1',
-     is_v_of_t v5 ->
-     reduce t1 t1' ->
-     reduce (t_App v5 t1) (t_App v5 t1')
-
-.
-
-(* progress *)
+Require Import List.
+Require Import STLC.stlc.
+Import ListNotations.
 
 Ltac caseEq f :=
-  generalize (refl_equal f); pattern f at -1; case f. 
+  generalize (refl_equal f); pattern f at -1; case f.
 
 Theorem progress:
   forall (t0:t) (T0:T),
     GtT nil t0 T0 ->
-    (is_v_of_t t0) \/ (exists t1, reduce t0 t1).
+    (is_v_of_t t0 = true) \/ (exists t1, reduce t0 t1).
 Proof.
   induction t0; intros T0 Ht.
 (* Case Var *) 
   inversion Ht; clear Ht; subst.
-  elim H1; clear H1; intros G1 H1.
-  elim H1; clear H1; intros G2 H1.
-  elim H1; clear H1; intros Ht1 Ht2.
-  cut (nil <> G1 ++ (t0, T0) :: G2).
+  case H1; clear H1; intros G1 H1.
+  case H1; clear H1; intros G2 H1.
+  case H1; clear H1; intros Ht1 Ht2.
+  cut ([] <> G1 ++ (x, T0) :: G2).
   2: apply app_cons_not_nil.
   intro Hc. rewrite Ht1 in Hc.
   contradiction Hc. trivial.
 (* Case Lam *)
-  left; red; trivial.
+  left; simpl; trivial.
 (* Case App *)
   right. inversion Ht; subst.
   elim IHt0_1 with (T0 := T_arrow T1 T0); 
@@ -145,30 +31,25 @@ Proof.
   caseEq t0_1; intros x t3; subst.
   (* want functional inversion over Ht0_1 instead of caseEq *)
   inversion H2; subst.
-  elim H1; clear H1; intros G1 H1.
-  elim H1; clear H1; intros G2 H1.
-  elim H1; clear H1; intros Ht1 Ht2.
-  cut (nil <> G1 ++ (x, T_arrow T1 T0) :: G2).
+  case H1; clear H1; intros G1 H1.
+  case H1; clear H1; intros G2 H1.
+  case H1; clear H1; intros Ht1 Ht2.
+  cut ([] <> G1 ++ (x, T_arrow T1 T0) :: G2).
   intro Hc. rewrite Ht1 in Hc.
   contradiction Hc. trivial.
   apply app_cons_not_nil.
   (**)
   intros; subst.
-  cut (is_v_of_t t0_2 \/ (exists t1 : t, reduce t0_2 t1)); eauto.
+  cut (is_v_of_t t0_2 = true \/ (exists t1 : t, reduce t0_2 t1)); eauto.
   intro. inversion H; clear H.
   generalize H0; clear H0.
   exists (tsubst_t t0_2 x t3).
-  apply ax_app. trivial.
-  elim H1. intro t1. intro H.
+  apply ax_app. rewrite H1. simpl. trivial.
+  case H1. intro t1. intro H.
   exists (t_App (t_Lam x t3) t1).
-  apply ctx_app_arg; trivial.
+  apply ctx_app_arg; simpl; trivial.
   (**)
   intro; subst.
-  cut (is_v_of_t t0_2 \/ (exists t1 : t, reduce t0_2 t1)); eauto.
-  intro; inversion H; clear H.
-  unfold is_v_of_t. intro. contradiction H.
-  elim H0; clear H0; intros t1 Ht1.
-  exists (t_App (t_App x t3) t1).
-  apply ctx_app_arg; trivial.
+  cut (is_v_of_t t0_2 = true \/ (exists t1 : t, reduce t0_2 t1)); eauto.
+  simpl; intros; congruence.
 Qed.
-  
